\chapter{DC Motor Control}
In application of DC Motor, we want to be able to control its position and angular velocity.

\section{Velocity Control using PI Control}
In this section we design a controller for dcmotor based on linearized dcmotor model using 2nd Order Differential Equation Design Workflow. From DC motor Model, we have:
\begin{equation}
	\label{dcmotorctrleq1}
	\dot{\omega}(t) = -a\omega(t) + bv_a(t) 	
\end{equation}
We have to design a velocity controller, thus the feedback of the system is angular velocity of the dc motor.\\
We have our PI control:
\begin{equation}
	\label{dcmotorctrleq2}
	v_a(t) = K_p(\omega_d(t) - \omega(t)) + K_i \int_{0}^{t} (\omega_d(t) - \omega(t)) \,dt
\end{equation}
From \autoref{dcmotorctrleq1},we get:
\begin{equation}
	\label{dcmotorctrleq3}
	v_a(t) = \frac{1}{b}\dot{\omega}_d(t) + \frac{a}{b}\omega_d(t)
\end{equation}
From \autoref{dcmotorctrleq2} and \autoref{dcmotorctrleq3}, we have our controller design:
\begin{equation}
	\label{dcmotorctrleq4}
	v_a(t) = \frac{1}{b}\dot{\omega}_d(t) + \frac{a}{b}\omega_d(t) + K_p(\omega_d(t) - \omega(t)) + K_i \int_{0}^{t} (\omega_d(t) - \omega(t)) \,dt
\end{equation}

\begin{figure}[h]
	\centering
	%\def\svgscale{1}
	\includesvg{src/dcmotorctrl/dcmotorctrl_fig1}
	\caption{Velocity Control PI Controller}
	\label{fig:Velocity Control PI Controller}
\end{figure}

Substitute \autoref{dcmotorctrleq4} back to model in \autoref{dcmotorctrleq1}, we get:
\begin{equation}
	\label{dcmotorctrleq5}
	\dot{\omega}(t) = -a\omega(t) + b\left(\frac{1}{b}\dot{\omega}_d(t) + \frac{a}{b}\omega_d(t) + K_p(\omega_d(t) - \omega(t)) + K_i \int_{0}^{t} (\omega_d(t) - \omega(t)) \,dt\right)
\end{equation}
\[
\begin{split}
	0 &= -\dot{\omega}(t) - a\omega(t) + \dot{\omega}_d(t) + a\omega_d(t) + bK_p(\omega_d(t) - \omega(t)) + bK_i \int_{0}^{t} (\omega_d(t) - \omega(t)) \,dt \\
	0 &= (\dot{\omega}_d(t) - \dot{\omega}(t)) + a(\omega_d(t) - \omega(t)) + bK_p(\omega_d(t) - \omega(t)) + bK_i \int_{0}^{t} (\omega_d(t) - \omega(t)) \,dt \\
	0 &= (\dot{\omega}_d(t) - \dot{\omega}(t)) + (a + bK_p)(\omega_d(t) - \omega(t)) + bK_i \int_{0}^{t} (\omega_d(t) - \omega(t)) \,dt \\
	0 &= \dot{e}_{\omega} + (a + bK_p)e_{\omega} + bK_i \int_{0}^{t} e_{\omega}\,dt \\
	0 &= \ddot{e}_{\omega} + (a + bK_p)\dot{e}_{\omega} + bK_ie_{\omega} \leftarrow \text{take derivative to cancel integral.}\\
\end{split}
\]
Thus, we get:
\begin{equation}
	\label{dcmotorctrleq6}
	\ddot{e}_{\omega} + (a + bK_p)\dot{e}_{\omega} + bK_ie_{\omega} = 0
\end{equation}
From 2nd Order differential equation standard form, we have:
\begin{equation}
	\label{dcmotorctrleq7}
	\ddot{X} + 2\zeta\omega_nX+\omega_n^2X = 0
\end{equation}
From \autoref{dcmotorctrleq6} and \autoref{dcmotorctrleq7}, we get:
\[
\begin{split}
	a + bK_p &= 2\zeta\omega_n \\
	bK_i     &= \omega_n^2 \\
	K_p      &= \frac{2\zeta\omega_n - a}{b} \\
	K_i      &= \frac{\omega_n^2}{b}
\end{split}
\]
From equation above, we want \(K_p > 0\). Thus, \(2\zeta\omega_n > a\), then \(\zeta\omega_n > \frac{a}{2}\) to ensure stability.

\begin{tcolorbox}[title=Velocity Control using PI Linear]
	\paragraph{Control input}
	\[v_a(t) = \frac{1}{b}\dot{\omega}_d(t) + \frac{a}{b}\omega_d(t) + K_p(\omega_d(t) - \omega(t)) + K_i \int_{0}^{t} (\omega_d(t) - \omega(t)) \,dt\]
	\paragraph{Control Tuning Constant}
	\[
	\begin{split}
		K_p      &= \frac{2\zeta\omega_n - a}{b} \\
		K_i      &= \frac{\omega_n^2}{b}
	\end{split}
	\]
\end{tcolorbox}

\section{Velocity Control using PID Control}
In this section we design a controller for dcmotor based on linearized dcmotor model using 2nd Order Differential Equation Design Workflow. From DC motor Model, We have our PID control:
\begin{equation}
	\label{dcmotorctrleq8}
	v_a(t) = K_p(\omega_d(t) - \omega(t)) + K_i \int_{0}^{t} (\omega_d(t) - \omega(t)) \,dt + K_d \frac{d}{dt} (\omega_d(t) - \omega(t))
\end{equation}
From \autoref{dcmotorctrleq3} and \autoref{dcmotorctrleq8}, we have our controller design:
\begin{equation}
	\label{dcmotorctrleq9}
	v_a(t) = \frac{1}{b}\dot{\omega}_d(t) + \frac{a}{b}\omega_d(t) + K_p(\omega_d(t) - \omega(t)) + K_i \int_{0}^{t} (\omega_d(t) - \omega(t)) \,dt + K_d \frac{d}{dt} (\omega_d(t) - \omega(t))
\end{equation}
Substitute \autoref{dcmotorctrleq9} back to model in \autoref{dcmotorctrleq1}, we get:
\begin{equation}
	\label{dcmotorctrleq10}
	\dot{\omega} = -a\omega + b\left(\frac{1}{b}\dot{\omega}_d + \frac{a}{b}\omega_d + K_p(\omega_d - \omega) + K_i \int_{0}^{t} (\omega_d - \omega) \,dt + K_d \frac{d}{dt} (\omega_d - \omega) \right)
\end{equation}
\[
\begin{split}
	0 &= -\dot{\omega} -a\omega + b(\frac{1}{b}\dot{\omega}_d + \frac{a}{b}\omega_d + K_p(\omega_d - \omega) + K_i \int_{0}^{t} (\omega_d - \omega) \,dt + K_d \frac{d}{dt} (\omega_d - \omega)) \\
	0 &= -\dot{\omega} -a\omega + \dot{\omega}_d + a\omega_d + bK_p(\omega_d - \omega) + bK_i \int_{0}^{t} (\omega_d - \omega) \,dt + bK_d \frac{d}{dt} (\omega_d - \omega) \\
	0 &= (\dot{\omega}_d -\dot{\omega}) + (a+bK_p)(\omega_d -\omega) + bK_i \int_{0}^{t} (\omega_d - \omega) \,dt + bK_d \frac{d}{dt} (\omega_d - \omega) \\
	0 &= (1+bK_d)(\dot{\omega}_d -\dot{\omega}) + (a+bK_p)(\omega_d -\omega) + bK_i \int_{0}^{t} (\omega_d - \omega) \,dt \\
	0 &= (1+bK_d)\dot{e}_{\omega} + (a+bK_p)e_{\omega} + bK_i \int_{0}^{t} e_{\omega} \,dt \\
	0 &= (1+bK_d)\ddot{e}_{\omega} + (a+bK_p)\dot{e}_{\omega} + bK_i e_{\omega} \\
\end{split}
\]
Thus, we get:
\begin{equation}
	\label{dcmotorctrleq11}
	\begin{split}
		(1+bK_d)\ddot{e}_{\omega} + (a+bK_p)\dot{e}_{\omega} + bK_ie_{\omega} = 0 \\
		\ddot{e}_{\omega} + \frac{(a+bK_p)}{(1+bK_d)}\dot{e}_{\omega} + \frac{bK_i}{(1+bK_d)} = 0
	\end{split}
\end{equation}
From 2nd Order differential equation standard form \autoref{dcmotorctrleq7}, we have:
\[
\begin{split}
	\frac{(a+bK_p)}{(1+bK_d)} &= 2\zeta\omega_n \\
	\frac{bK_i}{(1+bK_d)}     &= \omega_n^2 \\
\end{split}
\]

\begin{tcolorbox}[title=Velocity Control using PID Linear]
	\paragraph{Control input}
	\[v_a(t) = K_p(\omega_d(t) - \omega(t)) + K_i \int_{0}^{t} (\omega_d(t) - \omega(t)) \,dt + K_d \frac{d}{dt} (\omega_d(t) - \omega(t))\]
	\paragraph{Control Tuning Constant}
	We have more freedom to choose Kp Ki Kd, that satisfied :
	\[
	\begin{split}
		\frac{(a+bK_p)}{(1+bK_d)} &= 2\zeta\omega_n \\
		\frac{bK_i}{(1+bK_d)}     &= \omega_n^2 \\
	\end{split}
	\]
\end{tcolorbox}



\section{Position Control using PID Control}
In this section we design a controller for dcmotor based on linearized dcmotor model using 2nd/3rd Order Differential Equation Design Workflow. From DC motor Model, We have our PID control:
\begin{equation}
	\label{dcmotorctrleq12}
	v_a(t) = K_p(\theta_d(t) - \theta(t)) + K_i \int_{0}^{t} (\theta_d(t) - \theta(t)) \,dt + K_d \frac{d}{dt} (\theta_d(t) - \theta(t))
\end{equation}
From \autoref{dcmotorctrleq1}, it can be written in form of position as:
\begin{equation}
	\label{dcmotorctrleq13}
	\ddot{\theta}(t) = -a\dot{\theta}(t) + bv_a(t) 
\end{equation}
Thus, we get:
\begin{equation}
	\label{dcmotorctrleq14}
	v_a(t) = \frac{1}{b}\ddot{\theta}_d(t) + \frac{a}{b}\dot{\theta}_d(t)
\end{equation}
From \autoref{dcmotorctrleq13} and \autoref{dcmotorctrleq14}, we have our controller design:
\begin{equation}
	\label{dcmotorctrleq15}
	v_a(t) = \frac{1}{b}\ddot{\theta}_d(t) + \frac{a}{b}\dot{\theta}_d(t) + K_p(\theta_d(t) - \theta(t)) + K_i \int_{0}^{t} (\theta_d(t) - \theta(t)) \,dt + K_d \frac{d}{dt} (\theta_d(t) - \theta(t))
\end{equation}
Substitute \autoref{dcmotorctrleq15} to \autoref{dcmotorctrleq13}, we get:
\begin{equation}
	\label{dcmotorctrleq16}
	\ddot{\theta} = -a\dot{\theta} + b\left(\frac{1}{b}\ddot{\theta}_d + \frac{a}{b}\dot{\theta}_d + K_p(\theta_d - \theta) + K_i \int_{0}^{t} (\theta_d - \theta) \,dt + K_d \frac{d}{dt} (\theta_d - \theta)\right)
\end{equation}
\[
\begin{split}
	\ddot{\theta} &= -a\dot{\theta} + \ddot{\theta}_d + a\dot{\theta}_d + bK_p(\theta_d - \theta) + bK_i \int_{0}^{t} (\theta_d - \theta) \,dt + bK_d \frac{d}{dt} (\theta_d - \theta) \\
	0 &= -\ddot{\theta} -a\dot{\theta} + \ddot{\theta}_d + a\dot{\theta}_d + bK_p(\theta_d - \theta) + bK_i \int_{0}^{t} (\theta_d - \theta) \,dt + bK_d \frac{d}{dt} (\theta_d - \theta) \\
	0 &= (\ddot{\theta}_d -\ddot{\theta}) +a(\dot{\theta}_d -\dot{\theta}) + bK_p(\theta_d - \theta) + bK_i \int_{0}^{t} (\theta_d - \theta) \,dt + bK_d (\dot{\theta}_d -\dot{\theta}) \\
	0 &= (\ddot{\theta}_d -\ddot{\theta}) +(a+bK_d)(\dot{\theta}_d -\dot{\theta}) + bK_p(\theta_d - \theta) + bK_i \int_{0}^{t} (\theta_d - \theta) \,dt \\
	0 &= \ddot{e}_{\theta} +(a+bK_d) \dot{e}_{\theta} + bK_pe_{\theta} + bK_i \int_{0}^{t} e_{\theta} \,dt \\
	0 &= \dddot{e}_{\theta} +(a+bK_d) \ddot{e}_{\theta} + bK_p\dot{e}_{\theta} + bK_ie_{\theta} \\
\end{split}
\]
Thus, we get:
\begin{equation}
	\label{dcmotorctrleq17}
	\dddot{e}_{\theta} +(a+bK_d) \ddot{e}_{\theta} + bK_p\dot{e}_{\theta} + bK_ie_{\theta} = 0
\end{equation}
is the 3rd order differential equation with the characteristic form of:
\begin{equation}
	\label{dcmotorctrleq18}
	\lambda^3 + (a+bK_d)\lambda^2 + bK_p\lambda + bK_i = 0
\end{equation}
From \autoref{dcmotorctrleq18}, we know that in 3rd order differential equation characteristic polynomial, there exist 3 roots and at least 1 root is real root (denoted by $\lambda_1$).Thus, we can write:
\begin{equation}
	\label{dcmotorctrleq19}
	\begin{split}
		(\lambda + \lambda_1)(\lambda^2 + 2\zeta\omega_n\lambda + \omega_n^2) &= 0 \\
		\lambda^3 + 2\zeta\omega_n\lambda^2 + \omega_n^2\lambda + \lambda_1\lambda^2 + 2\zeta\omega_n\lambda\lambda_1 + \omega_n^2\lambda_1 &= 0 \\
		\lambda^3 + (2\zeta\omega_n + \lambda_1)\lambda^2 + (2\zeta\omega_n\lambda_1 + \omega_n^2)\lambda + \omega_n^2\lambda_1 &= 0
	\end{split}
\end{equation}
From \autoref{dcmotorctrleq18} and \autoref{dcmotorctrleq19}, we have:
\[\begin{split}
	a+bK_d &= 2\zeta\omega_n + \lambda_1 \\
	bK_p &= 2\zeta\omega_n\lambda_1 + \omega_n^2 \\
	bK_i &= \omega_n^2\lambda_1 \\
	K_d &= \frac{2\zeta\omega_n + \lambda_1 - a}{b} \\
	K_p &= \frac{2\zeta\omega_n\lambda_1 + \omega_n^2}{b} \\
	K_i &= \frac{\omega_n^2\lambda_1}{b}
\end{split}\]


\begin{tcolorbox}[title=Velocity Control using PID Linear]
	\paragraph{Control input}
	\[v_a(t) = K_p(\theta_d(t) - \theta(t)) + K_i \int_{0}^{t} (\theta_d(t) - \theta(t)) \,dt + K_d \frac{d}{dt} (\theta_d(t) - \theta(t))\]
	\paragraph{Control Tuning Constant}
	\[\begin{split}
		K_d &= \frac{2\zeta\omega_n + \lambda_1 - a}{b} \\
		K_p &= \frac{2\zeta\omega_n\lambda_1 + \omega_n^2}{b} \\
		K_i &= \frac{\omega_n^2\lambda_1}{b}
	\end{split}\]
\end{tcolorbox}