\chapter{2nd Order ODE Standard Form}
This section, we study on system of 2nd Order ODE with Standard Form Natural Frequency and Damping Ratio.
\section{Spring Mass Damper Modeling}
(Free Body Diagram)

\[
\begin{split}
	-kx(t) - b\dot{x}(t) &= m\ddot{x}(t) \\
	m\ddot{x}(t) + kx(t) + b\dot{x}(t)&= 0 \\
	\ddot{x} + \frac{b}{m} \dot{x}+\frac{k}{m} x(t) &= 0
\end{split}
\]
Let have the differential model above to look like the General Standard Form of :
\[
\boxed{\ddot{x}(t)+2\zeta\omega_n\dot{x}(t)+\omega_n^2x(t)=0}
\]
Where :
\begin{itemize}
	\item $ \zeta $ is damping ratio
	\item $ \omega_n $ is natural frequency
\end{itemize}
Thus, we have :
\begin{itemize}
	\item $ \frac{b}{m} = 2\zeta\omega_n \rightarrow \zeta = \frac{b}{2\sqrt{km}}$ 
	\item $ \frac{k}{m} = \omega_n^2 \rightarrow \omega_n = \sqrt{\frac{k}{m}}$
\end{itemize}
Let solve the Standard Form $ x(t) $:
\[ 
\ddot{x}(t)+2\zeta\omega_n\dot{x}(t)+\omega_n^2x(t)=0 
\]
Using Laplace Transform :
\[ 
\begin{split}
	s^2 X(s) - sx(0) -  \dot{x}(0) + 2\zeta\omega_n(sX(s)-x(0)) + \omega_n^2X(s) = 0 \\
	s^2 X(s) - sx_0 -  \dot{x}_0 + 2\zeta\omega_n(sX(s)-x_0) + \omega_n^2X(s) = 0 \\
\end{split}
\]
\[ 
X(s) = \frac{sx_0 + \dot{x}_0 + 2\zeta\omega_nx_0}{s^2 + 2\zeta\omega_ns+\omega_n^2}
\]
Let Find the root of the Denominator of $ X(s) $. From solving the 2nd order quadratic formula, we have the root :
\[ 
s_{1,2} = \frac{-2\zeta\omega_n \pm \sqrt{(2\zeta\omega_n)^2 - 4\omega_n^2}}{2} = -\zeta\omega_n \pm \omega_n\sqrt{\zeta^2-1}
\]
From the root, we can see that there are 3 cases:
\begin{itemize}
	\item Distinct Real Root
	\item Double Real Root
	\item Complex Root
\end{itemize}


\subsection{Distinct Real Roots}
To have the Distinct Real Root Case, We need:
\[ 
\begin{split}
	(2\zeta\omega_n)^2 - 4\omega_n^2 &> 0 \\
	4\zeta^2\omega_n^2 - 4\omega_n^2 &> 0 \\
	4\omega_n^2 (\zeta^2 - 1) &> 0 \\
	(\zeta^2 - 1) &> 0 \\
	\zeta^2  &> 1 \\
	\zeta &> 1
\end{split}
\]
We get Over-damped Case from the damping ratio of $ \boxed{\zeta > 1} $


\subsection{Double Real Root}
To have the Double Real Root Case, We need:
\[ 
\begin{split}
	(2\zeta\omega_n)^2 - 4\omega_n^2 &= 0 \\
	4\zeta^2\omega_n^2 - 4\omega_n^2 &= 0 \\
	4\omega_n^2 (\zeta^2 - 1) &= 0 \\
	(\zeta^2 - 1) &= 0 \\
	\zeta^2  &= 1 \\
	\zeta &= 1
\end{split}
\]
We get Critically damped Case from the damping ratio of $ \boxed{\zeta = 1} $. From the mathematical perspective, the damping ratio is unity (1) mean Critically damped. Where some people from control perspective prefer the damping ratio of $ \frac{1}{\sqrt{2}} $ to be Critically damped.


\subsection{Complex Root}
To have the Complex Root Case, We need:
\[ 
\begin{split}
	(2\zeta\omega_n)^2 - 4\omega_n^2 &< 0 \\
	4\zeta^2\omega_n^2 - 4\omega_n^2 &< 0 \\
	4\omega_n^2 (\zeta^2 - 1) &< 0 \\
	(\zeta^2 - 1) &< 0 \\
	\zeta^2  &< 1 \\
	\zeta &< 1
\end{split}
\]

\section{Discussion of Each Cases}
\subsection{Over-damped Case ($ \zeta > 1$)}
Above equation can be written as:
\[ 
X(s) = \frac{sx_0 + \dot{x}_0 + 2\zeta\omega_nx_0}{s^2 + 2\zeta\omega_ns+\omega_n^2} = \frac{a_1}{s+r_1}+\frac{a_2}{s+r_2}
\]
After using Partial Fraction Decomposition, we get:
\[ 
a_1 = \frac{-\dot{x}_0 + x_0 (-\zeta \omega_n + \sqrt{(\zeta^2-1)\omega_n^2})}{2\sqrt{(\zeta^2-1)\omega_n^2}}
\]
\[ 
a_2 = \frac{\dot{x}_0 + x_0 (\zeta \omega_n + \sqrt{(\zeta^2-1)\omega_n^2})}{2\sqrt{(\zeta^2-1)\omega_n^2}}
\]
Thus the solution of differential equation $ \ddot{x}(t)+2\zeta\omega_n\dot{x}(t)+\omega_n^2x(t)=0  $ where $ x(0)=x_0, \dot{x}(0) = \dot{x}_0 $ is :
\[ 
x(t) = a_1e^{r_1t}+a_2e^{r_2t} 
\]
Where:
\[
\begin{split}
	a_1 &= \frac{-\dot{x}_0 + x_0 (-\zeta \omega_n + \sqrt{(\zeta^2-1)\omega_n^2})}{2\sqrt{(\zeta^2-1)\omega_n^2}} \\
	a_2 &= \frac{\dot{x}_0 + x_0 (\zeta \omega_n + \sqrt{(\zeta^2-1)\omega_n^2})}{2\sqrt{(\zeta^2-1)\omega_n^2}} \\
	r_1,r_2 &= -\zeta\omega_n \pm \omega_n\sqrt{\zeta^2-1}
\end{split} 
\]

\subsection{Critically damped Case ($ \zeta = 1$)}
We have the root : $ r_1,r_2 = -\zeta\omega_n \pm \omega_n\sqrt{\zeta^2-1} $\\
By substitute $ \zeta = 1 $, we get the root : 
\[ r_1,r_2 = -\omega_n \]
Above equation can be written as:
\[ 
X(s) = \frac{sx_0 + \dot{x}_0 + 2\zeta\omega_nx_0}{s^2 + 2\zeta\omega_ns+\omega_n^2} = \frac{a_1}{s+\omega_n}+\frac{a_2}{(s+\omega_n)^2}
\]
After using Partial Fraction Decomposition, we get:
\[ 
a_1 = x_0
\]
\[ 
a_2 = \dot{x}_0 + x_0\omega_n
\]
Thus the solution of differential equation $ \ddot{x}(t)+2\zeta\omega_n\dot{x}(t)+\omega_n^2x(t)=0  $ where $ x(0)=x_0, \dot{x}(0) = \dot{x}_0 $ is :
\[ 
x(t) = x_0e^{-\omega_nt}+te^{-\omega_nt}(\dot{x}_0+x_0\omega_n)
\]
Where:
\[
\begin{split}
	a_1 &= x_0\\
	a_2 &= \dot{x}_0 + x_0\omega_n
\end{split} 
\]


\subsection{Under damped Case ($ \zeta < 1$)}
We have the root : $ r_1,r_2 = -\zeta\omega_n \pm \omega_n\sqrt{\zeta^2-1} $\\
By modify the square root part, we get :
\[
\begin{split}
	r_1,r_2 &= -\zeta\omega_n \pm \omega_n\sqrt{-1(1-\zeta^2)} \\
	&= -\zeta\omega_n \pm \omega_n\sqrt{(1-\zeta^2)}\sqrt{-1} \\
	&= -\zeta\omega_n \pm \omega_n\sqrt{(1-\zeta^2)}i \\
\end{split}
\]
Let:
\[
\begin{split}
	\sigma &= \zeta\omega_n\\
	\omega_d &=\omega_n\sqrt{(1-\zeta^2)} \\
\end{split}
\]
We can write the root as :
\[
r_1,r_2 = -\sigma \pm \omega_d i
\]
Rewrite the root in form of :
\[
s^2 + 2\zeta\omega_ns+\omega_n^2 = (s+\alpha)^2+w_n^2
\]
We get :
\[
\begin{split}
	\alpha &= \zeta\omega_n\\
	\omega &= \sqrt{(1-\zeta^2)\omega_n^2} \\
\end{split}
\]
Above equation can be written as:
\[ 
X(s) = \frac{sx_0 + \dot{x}_0 + 2\zeta\omega_nx_0}{s^2 + 2\zeta\omega_ns+\omega_n^2} = \frac{sx_0 + \dot{x}_0 + 2\zeta\omega_nx_0}{(s+\alpha)^2+w_n^2}
\]
After using Partial Fraction Decomposition, The solution of differential equation $ \ddot{x}(t)+2\zeta\omega_n\dot{x}(t)+\omega_n^2x(t)=0  $ where $ x(0)=x_0, \dot{x}(0) = \dot{x}_0 $ is :
\[
x(t) = a cos(\omega t) + b sin(\omega t)
\]
Where:
\[
\begin{split}
	a &= x_0e^{-\alpha t}\\
	b &= \frac{\dot{x}_0 + x_0\zeta\omega_n}{\omega} e^{-\alpha t}\\
	\alpha &= \zeta\omega_n \\
	\omega &= \sqrt{(1-\zeta^2)\omega_n^2} \\
\end{split} 
\]
Or in simple form of :
\[
x(t) = A e^{-\zeta \omega_n t}cos(\omega_d t - \phi)
\]
Where:
\[
\begin{split}
	A &= \sqrt{x_0^2 + \frac{(\dot{x}_0 + x_0\zeta\omega_n)^2}{(1-\zeta^2)\omega_n^2}}\\
	\omega_d &= \omega_n\sqrt{(1-\zeta^2)} \\
	\phi & = atan2(\frac{\dot{x}_0 + x_0\zeta\omega_n}{\omega_n\sqrt{(1-\zeta^2)}},x_0)
\end{split} 
\]